coq/era_inv.v
@@ -61,7 +61,7 @@ Lemma era_lam0_invX Γ Δ A1 A2 A3 B C m1 m2 s1 s2 t :
   Γ ; Δ ⊢ Lam0 A1 m1 s1 ~ Lam0 A2 m2 s1 : C ->
   C === Pi0 A3 B s2 ->
   (A3 :: Γ) ⊢ B : Sort t ->
-  (A3 :: Γ) ; _: Δ ⊢ m1 ~ m2 : B.
+  (A3 :: Γ) ; _: Δ ⊢ m1 ~ m2 : B /\ A1 === A3.
 Proof with eauto.
   move e1:(Lam0 A1 m1 s1)=>n1.
   move e2:(Lam0 A2 m2 s1)=>n2 tyL.
@@ -69,7 +69,7 @@ Proof with eauto.
   { move=>Γ Δ A B m m' s k tym ihm A1 A2 A3 B0 m1 m2
       s1 s2 t[e1 e2 e3][e5 e6 _]; subst.
     move=>/pi0_inj[eq1[eq2 e]]tyB0; subst.
-    have wf:=sta_type_wf tyB0. inv wf.
+    have wf:=sta_type_wf tyB0. inv wf. split...
     apply: era_conv...
     apply: era_ctx_conv0.
     exact: (conv_sym eq1).
@@ -85,7 +85,7 @@ Lemma era_lam1_invX Γ Δ A1 A2 A3 B C m1 m2 s1 s2 t :
   Γ ; Δ ⊢ Lam1 A1 m1 s1 ~ Lam1 A2 m2 s1 : C ->
   C === Pi1 A3 B s2 ->
   (A3 :: Γ) ⊢ B : Sort t ->
-  exists r, (A3 :: Γ) ; A3 :{r} Δ ⊢ m1 ~ m2 : B.
+  exists r, (A3 :: Γ) ; A3 :{r} Δ ⊢ m1 ~ m2 : B /\ A1 === A3.
 Proof with eauto.
   move e1:(Lam1 A1 m1 s1)=>n1.
   move e2:(Lam1 A2 m2 s1)=>n2 tyL.
@@ -99,7 +99,7 @@ Proof with eauto.
     have tyA0t:=sta_rd H4 rd1.
     have tyA0s:=sta_rd H3 rd2.
     have e:=sta_unicity tyA0t tyA0s. subst.
-    exists s.
+    exists s. split...
     apply: era_ctx_conv1.
     apply: conv_sym...
     exact: H3.
@@ -112,8 +112,8 @@ Proof with eauto.
 Qed.
 
 Lemma era_lam0_inv Γ Δ m m' A1 A2 A3 B s1 s2 :
-  Γ ; Δ ⊢ Lam0 A2 m s2 ~ Lam0 A3 m' s2 : Pi0 A1 B s1 ->
-  (A1 :: Γ) ; _: Δ ⊢ m ~ m' : B.
+  Γ ; Δ ⊢ Lam0 A1 m s2 ~ Lam0 A2 m' s2 : Pi0 A3 B s1 ->
+  (A3 :: Γ) ; _: Δ ⊢ m ~ m' : B /\ A1 === A3.
 Proof with eauto.
   move=>ty.
   have[t/sta_pi0_inv[r[tyB _]]]:=dyn_valid (era_dyn_type ty).
@@ -121,8 +121,8 @@ Proof with eauto.
 Qed.
 
 Lemma era_lam1_inv Γ Δ m m' A1 A2 A3 B s1 s2 :
-  Γ ; Δ ⊢ Lam1 A2 m s2 ~ Lam1 A3 m' s2 : Pi1 A1 B s1 ->
-  exists r, (A1 :: Γ) ; A1 :{r} Δ ⊢ m ~ m' : B.
+  Γ ; Δ ⊢ Lam1 A1 m s2 ~ Lam1 A2 m' s2 : Pi1 A3 B s1 ->
+  exists r, (A3 :: Γ) ; A3 :{r} Δ ⊢ m ~ m' : B /\ A1 === A3.
 Proof with eauto.
   move=>ty.
   have[t/sta_pi1_inv[r[tyB _]]]:=dyn_valid (era_dyn_type ty).
